Imp/features/exp_lam.v
@@ -1,4 +1,5 @@
 From Imp Require Export header_extensible.
+From Stdlib Require Import Lia.
 
 Section exp_lam.
     Variable exp : Type.
@@ -24,16 +25,51 @@ Section exp_lam.
             | ab t       => ab_ (open_rec (S k) u t)
         end.
 
+    Variable retract_open_rec : forall (n : nat) s (e : exp_lam),
+            open_rec n s (inj e) = open_rec_lam n s e.
+
     Variable lc' : nat -> exp -> Prop.
+    Variable open_rec_lc : forall s t n, lc' 0 s -> lc' (S n) t -> lc' n (open_rec n s t).
+    Variable lc_weaken   : forall s n m, n <= m  -> lc' n s -> lc' m s.
 
     Inductive lc'_lam : nat -> exp -> Prop := 
         | lc_app  n t t' : lc' n t -> lc' n t' -> lc'_lam n (app_ t t')
         | lc_ab   n t    : lc' (S n) t  -> lc'_lam n (ab_ t)
-        | lc_bvar k n    : n < k -> lc'_lam n (bvar_ k)
+        | lc_bvar k n    : k < n -> lc'_lam n (bvar_ k)
     .
 
     Variable retract_lc: forall n e, lc'_lam n e -> lc' n e.
     Variable retract_lc_rev: forall n e, lc' n (inj e) -> lc'_lam n (inj e).
+
+    Lemma nat_shenenigans : forall n m, n < S m -> n = m \/ n < m.
+    Proof. 
+        intros n. 
+        induction n.
+        - intros m. destruct m. {left. easy. } right. apply PeanoNat.Nat.lt_0_succ.
+        - intros m H'. apply PeanoNat.lt_S_n in H'.
+          destruct m. {apply PeanoNat.Nat.nlt_0_r in H'. exfalso. easy. }
+          apply IHn in H'. destruct H' as [-> |  H']. {left. easy. }
+          right. rewrite <- PeanoNat.Nat.succ_lt_mono. easy.
+    Qed.
+
+    Definition open_rec_lc_lam : forall s t n, lc' 0 s -> lc'_lam (S n) t -> lc' n (open_rec n s t).
+    Proof.
+    intros s t n H1 H2.
+    inversion H2.
+    - subst. unfold app_. rewrite retract_open_rec.
+      simpl. apply retract_lc.
+      constructor; apply open_rec_lc; try easy.
+    - unfold ab_. rewrite retract_open_rec.
+      simpl. apply retract_lc. constructor.
+      subst. apply open_rec_lc; try easy.
+    - subst. unfold bvar_. rewrite retract_open_rec. simpl.
+      destruct (nat_shenenigans k n). { easy. }
+      + subst. rewrite PeanoNat.Nat.eqb_refl. 
+        apply lc_weaken with (n := 0). lia. easy.
+      + destruct (Nat.eqb n k) eqn:n_eq_k.
+        { apply lc_weaken with (n:=0). lia. easy. }
+        apply retract_lc. constructor. easy.
+    Defined.    
 
     Variable value : exp -> Prop.
 
@@ -48,23 +84,33 @@ Section exp_lam.
     
 
     Inductive step_lam : Ctx -> exp -> Ctx -> exp -> Prop :=
-        | stepBeta   ctx s         t : value t -> step_lam ctx (app_ (ab_ s) t) ctx (open_rec 0 s t)
+        | stepBeta   ctx s         t : value t -> step_lam ctx (app_ (ab_ s) t) ctx (open_rec 0 t s)
         | stepAppL   ctx s ctx' s' t : value t -> step ctx s ctx' s' -> step_lam ctx (app_ s t) ctx' (app_ s' t)
         | stepAppR s ctx t ctx' t'   : step ctx t ctx' t' -> step_lam ctx (app_ s t) ctx' (app_ s t')
     .
 
+    Lemma lc_ab_inv : forall s n, lc' n (ab_ s) -> lc' (S n) s.
+    intros s n Hlc.
+    apply retract_lc_rev in Hlc. inversion Hlc; subst; try (apply retract_inj in H0; easy).
+    apply retract_inj in H0. inversion H0. subst. easy.
+    Qed.
 
-    Lemma preservation_lam : forall c e c' e', lc' 0 e -> step_lam c e c' e' -> lc' 0 e'.
+
+    Definition preservation_lam : forall c e c' e', lc' 0 e -> step_lam c e c' e' -> lc' 0 e'.
     Proof.
         intros c e c' e' lc_e.
         induction 1.
-        - apply retract_lc_rev in lc_e. inversion lc_e.
-            + apply retract_inj in H1. inversion H1. subst. clear H1.
-              
-              
-          
-        
-    Admitted.
+        - apply retract_lc_rev in lc_e. inversion lc_e; try (apply retract_inj in H1; easy).
+          apply retract_inj in H1. inversion H1. subst.
+          apply open_rec_lc; try easy.
+          apply lc_ab_inv. easy.
+        - apply retract_lc_rev in lc_e. inversion lc_e; try (apply retract_inj in H2; easy).
+          apply retract_inj in H2. inversion H2; subst; try (apply retract_inj in H2; easy).
+          apply retract_lc. constructor; try easy. apply (preservation ctx s ctx' s'); easy.
+        - apply retract_lc_rev in lc_e. inversion lc_e; try (apply retract_inj in H1; easy).
+          subst. apply retract_inj in H1. inversion H1. subst.
+          apply retract_lc. constructor. {easy. } 
+          apply (preservation ctx t ctx' t'); easy.      
+    Defined.
     
 End exp_lam.
-
